hpaxos_liveness.thy
@@ -1,0 +1,49 @@
+theory hpaxos_liveness
+imports Main hpaxos hpaxos_safety
+begin
+
+fun Termination_lrn :: "(nat \<Rightarrow> State) \<Rightarrow> Learner \<Rightarrow> bool" where
+  "Termination_lrn f l = (\<exists>n :: nat. \<exists>b :: Ballot. decision (f n) l b \<noteq> {})"
+
+fun Termination :: "(nat \<Rightarrow> State) \<Rightarrow> bool" where
+  "Termination f = 
+     (\<forall>l :: Learner.  
+        (\<exists>Q :: Acceptor set. Q \<subseteq> {x . is_safe x} \<and> TrustLive l Q) \<longrightarrow>
+        Termination_lrn f l)"
+
+(*Extract consecutive runs of given lengths from a stream*)
+fun sequence_of_runs :: "nat \<Rightarrow> nat list \<Rightarrow> (nat \<Rightarrow> 'a) \<Rightarrow> ('a list) list" where
+  "sequence_of_runs start [] f = []" |
+  "sequence_of_runs start (len # lens) f = 
+    map f [start ..< start + len] # sequence_of_runs (start + len) lens f"
+
+lemma sequence_of_runs_length_invar:
+  shows "\<forall> start1 start2 f1 f2. 
+           length (sequence_of_runs start1 lens f1) 
+           = length (sequence_of_runs start2 lens f2)"
+proof (induction lens; simp) qed
+
+theorem sequence_of_runs_length:
+  shows "length (sequence_of_runs start lens f) = length lens"
+proof (induction lens)
+  case Nil
+  then show ?case by simp
+next
+  case (Cons a lens)
+  then show ?case 
+    by (metis length_Cons sequence_of_runs.simps(2) sequence_of_runs_length_invar)
+qed
+
+
+
+fun runs_assumption :: "(State list) list \<Rightarrow> bool" where
+  "runs_assumption runs = True"
+
+fun network_assumption :: "(nat \<Rightarrow> State) \<Rightarrow> bool" where
+"network_assumption f = 
+    (\<exists>start lens. length lens = 13 \<and> (\<forall>i<13. lens ! i > 0) \<and> 
+                  runs_assumption (sequence_of_runs start lens f))"
+
+
+
+end
